Test/TreeStatsMain.lean
@@ -1,3 +1,7 @@
+-- SPDX-FileCopyrightText: 2026 Yuki Otsuka
+--
+-- SPDX-License-Identifier: BSD-3
+
 import Test.TreeStats
 
 def main (args : List String) : IO Unit :=
