ViE/Key.lean
@@ -1,3 +1,7 @@
+-- SPDX-FileCopyrightText: 2026 Yuki Otsuka
+--
+-- SPDX-License-Identifier: BSD-3
+
 import ViE.Key.Dispatch
 import ViE.Key.Map
 import ViE.Key.Input
