lakefile.lean
@@ -7,10 +7,13 @@ package vie where
   testDriver := "test"
 
 require bliku from git "https://github.com/4kusto/bliku" @ "main"
+require mathlib from git "https://github.com/leanprover-community/mathlib4.git"
 
 lean_lib ViE
 
 lean_lib Test
+
+lean_lib Proof
 
 @[default_target]
 lean_exe vie where
@@ -21,3 +24,6 @@ lean_exe test where
 
 lean_exe bench where
   root := `Test.Benchmark
+
+lean_exe proof where
+  root := `Proof.Main
