scripts/perf_bench_bin.sh
@@ -1,5 +1,9 @@
 #!/bin/bash
 
+# SPDX-FileCopyrightText: 2026 Yuki Otsuka
+#
+# SPDX-License-Identifier: BSD-3
+
 set -euo pipefail
 
 # Usage:
